\documentclass{article}
\usepackage{amsmath}

\begin{document}
  \begin{equation}
    \int\limits_{a}^{b} x\,dx = \left.\frac{x^2}{2}\right|_{a}^{b}
  \end{equation}

  \begin{equation}
    \iiint\limits_{V} f(x, y, z)\,dV = F
  \end{equation}

  \begin{equation}
    \frac{dx}{dy} = x\prime = \lim_{h \to 0} \frac{f(x+h)-f(x)}{h}
  \end{equation}

  \begin{equation}
    |x| = \begin{cases}
      -x, & \text{si } x < 0 \\
      x,  & \text{si } x \geq 0 \\
    \end{cases}
  \end{equation}

  \begin{equation}
    F(x) = A_0 + \sum_{n=1}^{N} \left[A_n \cos\left(\frac{2\pi nx}{P}\right) + B_n \sin\left(\frac{2\pi nx}{P}\right)\right]
  \end{equation}

  \begin{equation}
    \sum_{n} \frac{1}{n^s} = \prod_{p}\frac{1}{1 - \frac{1}{p^s}}
  \end{equation}

  \begin{equation}
    m\ddot{x} + c\dot{x} + kx = F_0 \sin(2\pi ft)
  \end{equation}
  
  \begin{align}
    \begin{split}
      f(x) \quad &= \quad x^2 + 3x + 5x^2 + 8 + 6x \\
           \quad &= \quad 6x^2 + 9x + 8 \\
           \quad &= \quad x(6x + 9) + 8 \\
    \end{split}
  \end{align}

  \begin{equation}
    X = \frac{F_0}{k}\frac{1}{\sqrt{(1 - r^2) + (2 \zeta r)^2}}
  \end{equation}

  \begin{equation}
    G_{\mu\nu} \equiv R_{\mu\nu} - \frac{1}{2}Rg_{\mu\nu} = \frac{8\pi G}{c^4}T_{\mu\nu}
  \end{equation}

  \begin{equation}
    6\text{CO}_2 + 6\text{H}_2\text{O} \rightarrow \text{C}_6\text{H}_{12}\text{O}_6 + 6\text{O}_2
  \end{equation}

  \begin{equation}
    \text{SO}_4^{2-} + \text{Ba}^{2+} \rightarrow \text{BaSO}_4
  \end{equation}
  \begin{equation}
    \begin{pmatrix}
      a_{11} & a_{12} & \ldots & a_{1n} \\
      a_{21} & a_{22} & \ldots & a_{2n} \\
      \vdots & \vdots & \ddots & \vdots \\
      a_{n1} & a_{n2} & \ldots & a_{nn} \\
    \end{pmatrix}
    \begin{pmatrix}
      v_1 \\
      v_2 \\
      \vdots \\
      v_n
    \end{pmatrix}
    =
    \begin{pmatrix}
      w_1 \\
      w_2 \\
      \vdots \\
      w_n      
    \end{pmatrix}
  \end{equation}

  \begin{equation}
    \frac{\partial \mathbf{u}}{\partial t} + (\mathbf{u} \cdot \nabla)\mathbf{u} - \nu\nabla^2(\mathbf{u}) = -\nabla \mathbf{h}
  \end{equation}

  \begin{equation}
    \alpha A \beta B \gamma\Gamma \delta\Delta \pi\Pi \omega\Omega
  \end{equation}
\end{document}